pushed through monads

src/ml/interpreter.ml
@@ -26,11 +26,11 @@ let rec step m =
   | Trace.Tau x -> step x
   | Trace.Ret v -> v
   | Trace.Err s -> failwith (Printf.sprintf "ERROR: %s" (Camlcoq.camlstring_of_coqstring s))
-  | Trace.Vis (IO.Call(t, f, args), k) ->
+  | Trace.Vis (IO.Call(m, t, f, args), k) ->
     (Printf.printf "UNINTERPRETED EXTERNAL CALL: %s - returning 0l to the caller\n" (Camlcoq.camlstring_of_coqstring f));
-    step (k (Obj.magic (DV.DVALUE_I64 DynamicValues.Int64.zero)))
+    step (k (Obj.magic (m, DV.DVALUE_I64 DynamicValues.Int64.zero)))
     
-  | Trace.Vis (IO.GEP(_, _, _), _) -> failwith "GEP failed"
+  | Trace.Vis (IO.GEP(_,_, _, _), _) -> failwith "GEP failed"
   | Trace.Vis _ -> failwith "should have been handled by the memory model"  
       
 
